Improve Unreachable Code.

theories/UnreachableCode.v
@@ -6,36 +6,75 @@ Set Implicit Arguments.
 
 Local Hint Resolve incl_empty minus_incl incl_right incl_left.
 
-Inductive sc := Sound | SoundAndComplete.
+Inductive sc := Sound | Complete | SoundAndComplete.
 
 Definition isComplete (s:sc) :=
   match s with
   | SoundAndComplete => true
+  | Complete => true
   | _ => false
   end.
+
+Definition isSound (s:sc) :=
+  match s with
+  | SoundAndComplete => true
+  | Sound => true
+  | _ => false
+  end.
+
+Definition uceq (i:sc) (a b:bool) :=
+  match i with
+  | Sound => impb a b
+  | Complete => impb b a
+  | SoundAndComplete => a = b
+  end.
+
+Hint Extern 0 (uceq _ _ _) => simpl.
+
+Lemma uceq_refl i a
+  : uceq i a a.
+Proof.
+  destruct i; simpl; eauto.
+Qed.
+
+Lemma eq_uceq i (a b:bool)
+  : a = b -> uceq i a b.
+Proof.
+  intros; subst. eauto using uceq_refl.
+Qed.
+
+Lemma eq_uceq_sym i (a b:bool)
+  : b = a -> uceq i a b.
+Proof.
+  intros; subst. eauto using uceq_refl.
+Qed.
+
+Hint Resolve uceq_refl eq_uceq eq_uceq_sym.
 
 Inductive unreachable_code (i:sc)
   : list bool -> stmt -> ann bool -> Prop :=
 | UCPOpr BL x s b e al
   :  unreachable_code i BL s al
-     -> getAnn al = b
+     -> uceq i b (getAnn al)
      -> unreachable_code i BL (stmtLet x e s) (ann1 b al)
 | UCPIf BL e b1 b2 b al1 al2
-  :  (op2bool e <> Some false -> getAnn al1 = b)
-     -> (op2bool e <> Some true -> getAnn al2 = b)
+  :  (op2bool e <> Some false -> uceq i b (getAnn al1))
+     -> (op2bool e <> Some true -> uceq i b (getAnn al2))
      -> unreachable_code i BL b1 al1
      -> unreachable_code i BL b2 al2
+     -> (if isComplete i then op2bool e = ⎣ false ⎦ -> getAnn al1 = false else True)
+     -> (if isComplete i then op2bool e = ⎣ true ⎦ -> getAnn al2 = false else True)
      -> unreachable_code i BL (stmtIf e b1 b2) (ann2 b al1 al2)
 | UCPGoto BL l Y b a
   : get BL (counted l) b
-    -> impb a b
+    -> (if isSound i then impb a b else True)
     -> unreachable_code i BL (stmtApp l Y) (ann0 a)
 | UCReturn BL e b
   : unreachable_code i BL (stmtReturn e) (ann0 b)
 | UCLet BL F t b als alt
   : unreachable_code i (getAnn ⊝ als ++ BL) t alt
     -> length F = length als
-    -> getAnn alt = b
+    -> uceq i b (getAnn alt)
     -> (forall n Zs a, get F n Zs ->
                  get als n a ->
                  unreachable_code i (getAnn ⊝ als ++ BL) (snd Zs) a)
@@ -43,16 +82,38 @@ Inductive unreachable_code (i:sc)
                                 get als n a ->
                                 getAnn a ->
                                 isCalledFrom trueIsCalled F t (LabI n)) else True)
+    -> (if isComplete i then forall n a, get als n a -> impb (getAnn a) b else True)
     -> unreachable_code i BL (stmtFun F t) (annF b als alt).
 
 Local Hint Extern 0 =>
 match goal with
-| [ H : op2bool ?e <> Some ?t , H' : op2bool ?e <> Some ?t -> ?B = ?C |- _ ] =>
+| [ H : op2bool ?e <> Some ?t , H' : op2bool ?e <> Some ?t -> _ |- _ ] =>
   specialize (H' H); subst
 end.
 
-Lemma unreachable_code_trueIsCalled i Lv s slv l
-  : unreachable_code i Lv s slv
+Lemma unreachable_code_SC_S Lv s slv
+  : unreachable_code SoundAndComplete Lv s slv
+    -> unreachable_code Sound Lv s slv.
+Proof.
+  intros UC.
+  general induction UC; simpl in *; subst; eauto 20 using unreachable_code, uceq_refl.
+  - econstructor; simpl; eauto using uceq_refl.
+  - econstructor; simpl; eauto using uceq_refl.
+Qed.
+
+Hint Resolve unreachable_code_SC_S.
+
+Lemma ucc_sound_and_complete BL s a
+  : unreachable_code Complete BL s a
+    -> unreachable_code Sound BL s a
+    -> unreachable_code SoundAndComplete BL s a.
+Proof.
+  intros UCC UCS.
+  general induction UCS; inv UCC; simpl in *; eauto 20 using unreachable_code, impb_eq.
+Qed.
+
+Lemma unreachable_code_trueIsCalled Lv s slv l
+  : unreachable_code Sound Lv s slv
     -> trueIsCalled s l
     -> exists b, get Lv (counted l) b /\ impb (getAnn slv) b.
 Proof.
@@ -60,19 +121,18 @@ Proof.
   revert Lv slv n.
   sind s; destruct s; intros Lv slv n UC IC; inv UC; inv IC;
     simpl in *; subst; simpl in *; eauto 20.
-  - (* eauto refuses to apply IH. *)
-    eapply (IH s); eauto.
-  - exploit (IH s1); eauto.
-  - exploit (IH s2); eauto.
+  - edestruct (IH s); dcr; eauto.
+  - edestruct (IH s1); dcr; eauto.
+  - edestruct (IH s2); dcr; eauto.
   - destruct l'.
     exploit (IH s); eauto; dcr.
-    setoid_rewrite H8.
-    clear H7 H6 UC H8 H1 alt.
-    general induction H3.
+    setoid_rewrite H3. setoid_rewrite H10.
+    clear H3 H10 UC H9 H1 alt.
+    general induction H5.
     + inv_get. eexists; split; eauto.
     + inv_get.
-      exploit H5; eauto.
-      eapply IH in H4; eauto.
+      exploit H4; eauto.
+      eapply IH in H3; eauto.
       dcr. inv_get.
       edestruct IHcallChain; try eapply H8; eauto; dcr.
       eexists x1; split; eauto.
